# Partialbruchzerlegung

$$

\frac{\color{blue}1}{(x-1)(x+1)}

=
\frac
{
    \color{green}A
}
{
    (x-1)
}
+
\frac
{
    \color{red}B
}
{
    (x+1)
}
\tag{ (x-1) (x+1)}

$$

$$
\color{blue}1
\color{black}=
\color{green}A
\color{black}
(x+1)
+
\color{red}B
\color{black}
(x-1)

\tag{ausformulieren}

$$


$$

\color{blue}1
\color{black}=
\color{green}A
\color{black}x
+ 
\color{green}A
\color{black}
+
\color{red}B
\color{black}x
-
\color{red}B
$$

$$

\color{blue}1
\color{black}=
(\color{green}A
\color{black}+
\color{red}B
\color{black})
+
(
    \color{green}A
    \color{black}-
    \color{red}B
\color{black})
$$

-> Gleichung muss **IMMER** stimmen
sommit gilt:
$$



\underbrace{(
    \color{green}A
    \color{black}+
    \color{red}B)
}_{0}

\cdot
x = 0

$$

$$

1 = 0 + \underbrace{(
    \color{green}A
    \color{black}-
    \color{red}B)
}_{1}

$$


$$
\rightarrow
\begin{vmatrix}
   A+B = 0 \\
   A-B =1
\end{vmatrix}

\rightarrow
A = \frac{1}{2},
B= -\frac{1}{2}
$$